add bedrock2.Scalars: separation logic for words

bedrock2/src/Examples/bsearch.v
@@ -1,5 +1,5 @@
 Require Import Coq.Strings.String Coq.ZArith.ZArith.
-From bedrock2 Require Import NotationsInConstr ProgramLogic Map.Separation Array TailRecursion.
+From bedrock2 Require Import NotationsInConstr ProgramLogic Map.Separation Array Scalars TailRecursion.
 
 Require bedrock2.Examples.Demos.
 Definition bsearch := @Demos.bsearch _ Demos.BinarySearch.StringNames.Inst.
@@ -8,99 +8,12 @@ From coqutil Require Import Word.Interface Map.Interface. (* coercions word and 
 From bedrock2 Require Import Semantics BasicC64Semantics.
 
 Import HList List.
-Definition littleendian (n : nat) (addr : word) (value : Z) : mem -> Prop :=
-  array ptsto (word.of_Z 1) addr (tuple.to_list (LittleEndian.split n value)).
-Definition scalar sz addr value : mem -> Prop :=
-  littleendian (bytes_per (width:=width) sz) addr (word.unsigned value).
-
-Lemma load_bytes_sep a n bs R m
-  (Hsep : sep (array ptsto (word.of_Z 1) a (tuple.to_list bs)) R m)
-  : Memory.load_bytes n m a = Some bs.
-Proof.
-  cbv [load_bytes footprint].
-  revert dependent a; revert dependent R; revert dependent m; revert dependent n.
-  induction n; [solve[cbn; intros []; trivial]|].
-  intros [b0 bs] m R a Hsep.
-  cbn in Hsep; eapply SeparationLogic.sep_assoc in Hsep.
-  cbn [map.getmany_of_tuple tuple.option_all tuple.map tuple.unfoldn].
-  erewrite SeparationLogic.get_sep by exact Hsep.
-  setoid_rewrite IHn; [exact eq_refl|].
-  cbn.
-  refine (Lift1Prop.subrelation_iff1_impl1 _ _ _ _ _ Hsep); clear Hsep.
-  SeparationLogic.ecancel.
-Admitted.
-
-Lemma combine_split n z :
- LittleEndian.combine n (LittleEndian.split n z) = (z mod 2^(Z.of_nat n*8))%Z.
-Proof.
-  revert z; induction n.
-  { cbn. intros. rewrite Z.mod_1_r. trivial. }
-  { cbn [LittleEndian.split LittleEndian.combine PrimitivePair.pair._1 PrimitivePair.pair._2]; intros.
-    erewrite IHn; clear IHn.
-    rewrite word.unsigned_of_Z, Nat2Z.inj_succ, Z.mul_succ_l by Lia.lia.
-    (* bitwise proof, automatable: *)
-    eapply Z.bits_inj'; intros i Hi.
-    repeat rewrite ?Z.lor_spec, ?Properties.Z.testbit_mod_pow2, ?Z.shiftl_spec, ?Z.shiftr_spec by Lia.lia.
-    destruct (Z.ltb_spec0 i 8); cbn [andb orb].
-    { rewrite (Z.testbit_neg_r _ (i-8)) by Lia.lia.
-      rewrite Bool.andb_false_r, Bool.orb_false_r.
-      destruct (Z.ltb_spec0 i (Z.of_nat n * 8 + 8)); trivial; Lia.lia. }
-    { rewrite Z.shiftr_spec by Lia.lia.
-      replace (i - 8 + 8)%Z with i by Lia.lia; f_equal.
-      destruct
-        (Z.ltb_spec0 (i-8) (Z.of_nat n * 8)),
-        (Z.ltb_spec0 i (Z.of_nat n * 8 + 8));
-        trivial; Lia.lia. } }
-Qed.
-
-Lemma load_sep sz addr value R m
-  (Hsep : sep (scalar sz addr value) R m)
-  : Memory.load sz m addr = Some (word.and value (word.of_Z (Z.ones (Z.of_nat (bytes_per (width:=width) sz)*8)))).
-Proof.
-  cbv [load scalar littleendian] in *.
-  erewrite load_bytes_sep by exact Hsep; apply f_equal.
-  eapply Properties.word.unsigned_inj.
-  rewrite combine_split.
-  rewrite word.unsigned_and.
-  rewrite !word.unsigned_of_Z.
-  set (x := (Z.of_nat (bytes_per sz) * 8)%Z).
-  assert ((0 <= x)%Z) by (subst x; destruct sz; Lia.lia).
-  (* bitwise proof, automatable: *)
-  eapply Z.bits_inj'; intros i Hi.
-  repeat rewrite ?Properties.Z.testbit_mod_pow2, ?Properties.Z.testbit_ones, ?Z.lor_spec, ?Z.shiftl_spec, ?Z.shiftr_spec, ?Z.land_spec by (cbn; Lia.lia).
-  repeat match goal with |- context[(?a <? ?b)%Z]
-                         => destruct (Z.ltb_spec0 a b)
-         end; try Btauto.btauto.
-  destruct (Z.leb_spec0 0 i); cbn; try Btauto.btauto.
-  Lia.lia.
-Qed.
-
-Lemma load_word_sep (sz := Syntax.access_size.word) addr value R m 
-  (Hsep : sep (scalar sz addr value) R m)
-  : Memory.load sz m addr = Some value.
-Proof.
-  erewrite load_sep by exact Hsep; f_equal.
-  cbv [bytes_per sz].
-  eapply Properties.word.unsigned_inj.
-  rewrite !word.unsigned_and, !word.unsigned_of_Z.
-  rewrite <-Properties.word.wrap_unsigned at 2.
-  eapply Z.bits_inj'; intros i Hi.
-  repeat rewrite ?Properties.Z.testbit_mod_pow2, ?Properties.Z.testbit_ones, ?Z.lor_spec, ?Z.shiftl_spec, ?Z.shiftr_spec, ?Z.land_spec by (cbn; Lia.lia).
-  destruct (Z.ltb_spec0 i width); cbn [andb]; trivial; [].
-  destruct (Z.testbit (word.unsigned value) i); cbn [andb]; trivial; [].
-  destruct (Z.leb_spec0 0 i); try Lia.lia; cbn [andb]; [].
-  eapply Z.ltb_lt.
-  pose proof (word.width_pos : (0 < width)%Z) as H; clear - l H.
-  rewrite Z2Nat.id.
-Admitted.
-
-Axiom ptsto_word :  word -> word -> mem -> Prop.
 Instance spec_of_bsearch : spec_of "bsearch"%string := fun functions =>
   forall left right target xs R t m,
-    sep (array ptsto_word (word.of_Z 4) left xs) R m ->
+    sep (array (scalar Syntax.access_size.word) (word.of_Z 8) left xs) R m ->
     WeakestPrecondition.call (fun _ => True) (fun _ => False) (fun _ _ => True) functions
       "bsearch"%string t m (left::right::target::nil)%list
-      (fun t' m' rets => t=t' /\ sep (array ptsto_word (word.of_Z 4) left xs) R m' /\ exists i, rets = (i::nil)%list /\
+      (fun t' m' rets => t=t' /\ sep (array (scalar Syntax.access_size.word) (word.of_Z 8) left xs) R m' /\ exists i, rets = (i::nil)%list /\
       ((*sorted*)False -> True)
       ).
 
@@ -118,7 +31,7 @@ Proof.
   refine (
     tailrec (HList.polymorphic_list.cons (list word) (HList.polymorphic_list.nil)) ("left"::"right"::"target"::nil)%list%string
         (fun l xs t m left right target => PrimitivePair.pair.mk
-          (List.length xs = l /\ sep (array ptsto_word (word.of_Z 4) left xs) R m)
+          (List.length xs = l /\ sep (array (scalar Syntax.access_size.word) (word.of_Z 8) left xs) R m)
         (fun      T M LEFT RIGHT TARGET => True))
         _ lt_wf _ _ _ _ _);
     
@@ -134,13 +47,18 @@ Proof.
   { admit. }
   { repeat straightline.
     (* TODO: fix seprewrite to actually rewrite not just factor *)
-    evar (i:word.rep).
     eapply SeparationLogic.Proper_sep_iff1 in H1.
     3:reflexivity.
     2:symmetry.
-    2:unshelve eapply (array_index_inbounds _ _ _ _ _ i _); shelve_unifiable.
-    4:let i := rdelta i in unify i (word.divu (word.sub v0 left) (word.of_Z 4)).
-    (* TODO: array rule:
-    forall size left, p-left < length -> p-left mod size = 0 ->
-    forall i, i = (p-left)/size -> *)
+    2:eapply (array_address_inbounds _ _ (word.of_Z 0) _ _ v0).
+    4:reflexivity.
+    3: {
+      subst v0.
+      cbn [interp_binop].
+      unshelve erewrite (_:forall x y, word.sub (word.add x y) x = y). admit.
+      rewrite word.unsigned_slu, Properties.word.unsigned_sru_nowrap by admit.
+      rewrite Z.shiftl_mul_pow2, Z.shiftr_div_pow2.
+      rewrite !word.unsigned_of_Z.
+      cbn.
+      set ((Naive.unsigned x1 - Naive.unsigned x0) mod 18446744073709551616 / 16)%Z.
 Abort All.
