bedrock2/src/Scalars.v
@@ -1,0 +1,101 @@
+Require Import coqutil.Map.Interface bedrock2.Map.Separation bedrock2.Map.SeparationLogic bedrock2.Lift1Prop bedrock2.Semantics bedrock2.Array coqutil.Word.LittleEndian.
+Require Import Coq.Lists.List Coq.ZArith.ZArith.
+Require Import coqutil.Word.Interface coqutil.Map.Interface. (* coercions word and rep *)
+Require Import coqutil.Z.div_mod_to_equations.
+Import HList List.
+
+Section Scalars.
+  Context {width : Z} {word : Word.Interface.word width} {word_ok : word.ok word}.
+  Context {byte : Word.Interface.word 8} {byte_ok : word.ok byte}.
+  Context {mem : map.map word byte} {mem_ok : map.ok mem}.
+
+  Definition littleendian (n : nat) (addr : word) (value : Z) : mem -> Prop :=
+    array ptsto (word.of_Z 1) addr (tuple.to_list (LittleEndian.split n value)).
+
+  (* TODO: this definition should also enforce that [value] fits
+    within the specified width. Further, it might be better to take [value] as a Z. *)
+  Definition scalar sz addr (value:word) : mem -> Prop :=
+    littleendian (bytes_per (width:=width) sz) addr (word.unsigned value).
+  
+  Lemma load_bytes_sep a n bs R m
+    (Hsep : sep (array ptsto (word.of_Z 1) a (tuple.to_list bs)) R m)
+    : Memory.load_bytes n m a = Some bs.
+  Proof.
+    cbv [load_bytes footprint].
+    revert dependent a; revert dependent R; revert dependent m; revert dependent n.
+    induction n; [solve[cbn; intros []; trivial]|].
+    intros [b0 bs] m R a Hsep.
+    cbn in Hsep; eapply SeparationLogic.sep_assoc in Hsep.
+    cbn [map.getmany_of_tuple tuple.option_all tuple.map tuple.unfoldn].
+    erewrite SeparationLogic.get_sep by exact Hsep.
+    setoid_rewrite IHn; [exact eq_refl|].
+    cbn.
+    refine (Lift1Prop.subrelation_iff1_impl1 _ _ _ _ _ Hsep); clear Hsep.
+    SeparationLogic.ecancel.
+  Qed.
+  
+  Lemma combine_split n z :
+   LittleEndian.combine n (LittleEndian.split n z) = (z mod 2^(Z.of_nat n*8))%Z.
+  Proof.
+    revert z; induction n.
+    { cbn. intros. rewrite Z.mod_1_r. trivial. }
+    { cbn [LittleEndian.split LittleEndian.combine PrimitivePair.pair._1 PrimitivePair.pair._2]; intros.
+      erewrite IHn; clear IHn.
+      rewrite word.unsigned_of_Z, Nat2Z.inj_succ, Z.mul_succ_l by Lia.lia.
+      (* bitwise proof, automatable: *)
+      eapply Z.bits_inj'; intros i Hi.
+      repeat rewrite ?Z.lor_spec, ?Properties.Z.testbit_mod_pow2, ?Z.shiftl_spec, ?Z.shiftr_spec by Lia.lia.
+      destruct (Z.ltb_spec0 i 8); cbn [andb orb].
+      { rewrite (Z.testbit_neg_r _ (i-8)) by Lia.lia.
+        rewrite Bool.andb_false_r, Bool.orb_false_r.
+        destruct (Z.ltb_spec0 i (Z.of_nat n * 8 + 8)); trivial; Lia.lia. }
+      { rewrite Z.shiftr_spec by Lia.lia.
+        replace (i - 8 + 8)%Z with i by Lia.lia; f_equal.
+        destruct
+          (Z.ltb_spec0 (i-8) (Z.of_nat n * 8)),
+          (Z.ltb_spec0 i (Z.of_nat n * 8 + 8));
+          trivial; Lia.lia. } }
+  Qed.
+  
+  Lemma load_sep sz addr (value:word) R m
+    (Hsep : sep (scalar sz addr value) R m)
+    : Memory.load sz m addr = Some (word.and value (word.of_Z (Z.ones (Z.of_nat (bytes_per (width:=width) sz)*8)))).
+  Proof.
+    cbv [load scalar littleendian] in *.
+    erewrite load_bytes_sep by exact Hsep; apply f_equal.
+    eapply Properties.word.unsigned_inj.
+    rewrite combine_split.
+    rewrite word.unsigned_and.
+    rewrite !word.unsigned_of_Z.
+    set (x := (Z.of_nat (bytes_per sz) * 8)%Z).
+    assert ((0 <= x)%Z) by (subst x; destruct sz; Lia.lia).
+    (* bitwise proof, automatable: *)
+    eapply Z.bits_inj'; intros i Hi.
+    pose proof word.width_pos (width:=width).
+    repeat rewrite ?Properties.Z.testbit_mod_pow2, ?Properties.Z.testbit_ones, ?Z.lor_spec, ?Z.shiftl_spec, ?Z.shiftr_spec, ?Z.land_spec by Lia.lia.
+    repeat match goal with |- context[(?a <? ?b)%Z]
+                           => destruct (Z.ltb_spec0 a b)
+           end; try Btauto.btauto.
+    destruct (Z.leb_spec0 0 i); cbn; try Btauto.btauto.
+    Lia.lia.
+  Qed.
+  
+  Lemma load_word_sep (sz := Syntax.access_size.word) addr value R m 
+    (Hsep : sep (scalar sz addr value) R m)
+    : Memory.load sz m addr = Some value.
+  Proof.
+    erewrite load_sep by exact Hsep; f_equal.
+    cbv [bytes_per sz].
+    eapply Properties.word.unsigned_inj.
+    rewrite !word.unsigned_and, !word.unsigned_of_Z.
+    rewrite <-Properties.word.wrap_unsigned at 2.
+    eapply Z.bits_inj'; intros i Hi.
+    pose proof word.width_pos (width:=width).
+    repeat rewrite ?Properties.Z.testbit_mod_pow2, ?Properties.Z.testbit_ones, ?Z.lor_spec, ?Z.shiftl_spec, ?Z.shiftr_spec, ?Z.land_spec by Lia.lia.
+    destruct (Z.ltb_spec0 i width); cbn [andb]; trivial; [].
+    destruct (Z.testbit (word.unsigned value) i); cbn [andb]; trivial; [].
+    destruct (Z.leb_spec0 0 i); try Lia.lia; cbn [andb]; [].
+    eapply Z.ltb_lt.
+    rewrite Z2Nat.id; Z.div_mod_to_equations; Lia.nia.
+  Qed.
+End Scalars.
